Updated the examples

examples/BuildingEntry.thy
@@ -54,17 +54,17 @@ zoperation CEnterBuilding =
   update "[l \<leadsto> l @ [p]]"
 
 definition ListRetrieveSet :: "CSystem \<Rightarrow> (_, ASystem) itree" where
-"ListRetrieveSet = \<questiondown>CSystem? \<Zcomp> \<langle>\<lblot>s \<leadsto> set l\<rblot>\<rangle>\<^sub>a"
+"ListRetrieveSet = \<questiondown>CSystem? ;; \<langle>\<lblot>s \<leadsto> set l\<rblot>\<rangle>\<^sub>a"
 
 definition SetRetrieveList :: "ASystem \<Rightarrow> (_, CSystem) itree" where
-"SetRetrieveList = \<questiondown>ASystem? \<Zcomp> \<langle>\<lblot>l \<leadsto> sorted_list_of_set s\<rblot>\<rangle>\<^sub>a"
+"SetRetrieveList = \<questiondown>ASystem? ;; \<langle>\<lblot>l \<leadsto> sorted_list_of_set s\<rblot>\<rangle>\<^sub>a"
 
 find_theorems "(\<circ>\<^sub>s)"
 
-lemma "ListRetrieveSet \<Zcomp> SetRetrieveList = \<questiondown>CSystem?"
+lemma "ListRetrieveSet ;; SetRetrieveList = \<questiondown>CSystem?"
   apply (simp add: ListRetrieveSet_def SetRetrieveList_def ASystem_inv_def assigns_seq kcomp_assoc assigns_assume assigns_seq_comp usubst usubst_eval)
 
-lemma "p \<in> Staff \<Longrightarrow> (ListRetrieveSet \<Zcomp> AEnterBuilding p) \<sqsubseteq> (CEnterBuilding p \<Zcomp> ListRetrieveSet)"
+lemma "p \<in> Staff \<Longrightarrow> (ListRetrieveSet ;; AEnterBuilding p) \<sqsubseteq> (CEnterBuilding p ;; ListRetrieveSet)"
   unfolding ListRetrieveSet_def AEnterBuilding_def CEnterBuilding_def
   apply refine_auto
    apply (simp add: distinct_card)
