examples/Incubator.thy
@@ -13,35 +13,33 @@ def_consts
   MAX_TEMP = 30
   MIN_TEMP = 15
 
-schema IncubatorMonitor = 
+zstore IncubatorMonitor = 
   temp :: \<int>
   where "MIN_TEMP \<le> temp" "temp \<le> MAX_TEMP"
-
-record_default IncubatorMonitor
 
 zoperation Increment =
   over IncubatorMonitor
   pre "temp < MAX_TEMP"
   update "[temp\<Zprime> = temp + 1]"
 
-lemma Increment_correct: "\<^bold>{IncubatorMonitor\<^bold>} Increment() \<^bold>{IncubatorMonitor\<^bold>}"
-  unfolding Increment_def IncubatorMonitor_inv_def by hoare_wlp
+lemma Increment_correct: "\<^bold>{IncubatorMonitor_inv\<^bold>} Increment() \<^bold>{IncubatorMonitor_inv\<^bold>}"
+  by zpog_full
 
 zoperation Decrement =
   over IncubatorMonitor
   pre "temp > MIN_TEMP" \<comment> \<open> Change to @{term "(temp \<ge> MIN_TEMP)\<^sub>e"} to break the invariant \<close>
   update "[temp\<Zprime> = temp - 1]"
 
-lemma Decrement_correct: "\<^bold>{IncubatorMonitor\<^bold>} Decrement() \<^bold>{IncubatorMonitor\<^bold>}"
-  unfolding Decrement_def IncubatorMonitor_inv_def by hoare_wlp
+lemma Decrement_correct: "\<^bold>{IncubatorMonitor_inv\<^bold>} Decrement() \<^bold>{IncubatorMonitor_inv\<^bold>}"
+  by zpog_full
 
 zoperation GetTemp =
   over IncubatorMonitor
   params currentTemp \<in> TEMP
   where "temp = currentTemp"
 
-lemma GetTemp_correct: "\<^bold>{IncubatorMonitor\<^bold>} GetTemp v \<^bold>{IncubatorMonitor\<^bold>}"
-  unfolding GetTemp_def IncubatorMonitor_inv_def by hoare_wlp
+lemma GetTemp_correct: "\<^bold>{IncubatorMonitor_inv\<^bold>} GetTemp v \<^bold>{IncubatorMonitor_inv\<^bold>}"
+  by zpog_full
 
 zmachine Incubator =
   init "[temp \<leadsto> 20]"
